end2end/src/end2end/MetricLightbulbInvariant.v
@@ -1,0 +1,167 @@
+Require Import String.
+Require Import Coq.ZArith.ZArith.
+Require Import coqutil.Z.Lia.
+Require Import Coq.Lists.List. Import ListNotations.
+Require Import Coq.Logic.FunctionalExtensionality.
+Require Import coqutil.Word.LittleEndian.
+Require Import coqutil.Word.Properties.
+Require Import coqutil.Map.Interface.
+Require Import coqutil.Tactics.Tactics.
+Require Import coqutil.Datatypes.PropSet.
+Require Import compiler.RunInstruction.
+Require Import compiler.RiscvEventLoop.
+Require Import compiler.ForeverSafe.
+Require Import compiler.GoFlatToRiscv.
+Require Import coqutil.Tactics.Simp.
+Require Import bedrock2.Syntax bedrock2.Semantics.
+Require Import compiler.Pipeline.
+Require Import compilerExamples.MMIO.
+Require Import compiler.FlatToRiscvDef.
+Require Import bedrock2.WeakestPreconditionProperties.
+Require Import compiler.SeparationLogic.
+Require Import compiler.ToplevelLoop.
+Require Import compiler.CompilerInvariant.
+Require Import compiler.ExprImpEventLoopSpec.
+Require Import Coq.Classes.Morphisms.
+Require Import coqutil.Macros.WithBaseName.
+Require Import bedrock2Examples.metric_lightbulb.
+Require Import bedrock2Examples.lightbulb_spec.
+From coqutil Require Import SortedListWord.
+From bedrock2 Require Import Syntax NotationsCustomEntry. Import Syntax.Coercions.
+From compiler Require Import Symbols.
+Local Open Scope Z_scope.
+
+From coqutil Require Import Word.Naive.
+Require Import coqutil.Word.Bitwidth32.
+#[local] Existing Instance Naive.word.
+#[local] Existing Instance Naive.word32_ok.
+#[local] Existing Instance SortedListString.map.
+#[local] Existing Instance SortedListString.ok.
+#[local] Existing Instance SortedListWord.ok.
+#[local] Existing Instance SortedListWord.map.
+#[local] Instance : FlatToRiscvCommon.bitwidth_iset 32 Decode.RV32IM := eq_refl.
+
+Definition ml : MemoryLayout (width:=32) := {|
+  code_start    := word.of_Z 0;
+  code_pastend  := word.of_Z (2 ^ 12);
+  heap_start    := word.of_Z (2 ^ 12);
+  heap_pastend  := word.of_Z (2 ^ 12 + 2 ^ 11);
+  stack_start   := word.of_Z (2 ^ 12 + 2 ^ 11);
+  stack_pastend := word.of_Z (2 ^ 13);
+|}.
+Definition buffer_addr: Z := word.unsigned ml.(heap_start).
+
+Lemma ml_ok : MemoryLayout.MemoryLayoutOk ml. Proof. split; cbv; trivial; inversion 1. Qed.
+
+Definition init := func! { lightbulb_init() } .
+Definition loop := func! { unpack! _err = lightbulb_loop() } .
+Definition funcs := &[,init; loop] ++ map.tuples function_impls.
+
+Derive lightbulb_compiler_result SuchThat
+  (ToplevelLoop.compile_prog (string_keyed_map:=@SortedListString.map) MMIO.compile_ext_call ml funcs
+  = Success lightbulb_compiler_result)
+  As lightbulb_compiler_result_ok.
+Proof.
+  match goal with x := _ |- _ => cbv delta [x]; clear x end.
+  vm_compute.
+  match goal with |- @Success ?A ?x = Success ?e => is_evar e;
+    exact (@eq_refl (result A) (@Success A x)) end.
+Qed. Optimize Heap.
+
+Definition lightbulb_stack_size := snd lightbulb_compiler_result.
+Definition lightbulb_finfo := snd (fst lightbulb_compiler_result).
+Definition lightbulb_insns := fst (fst lightbulb_compiler_result).
+Definition lightbulb_bytes := Pipeline.instrencode lightbulb_insns.
+Definition lightbulb_symbols : list byte := Symbols.symbols lightbulb_finfo.
+
+Lemma compiler_emitted_valid_instructions :
+  bverify.bvalidInstructions Decode.RV32IM lightbulb_insns = true.
+Proof. vm_cast_no_check (eq_refl true). Qed.
+
+Require Import compiler.CompilerInvariant.
+Require Import compiler.NaiveRiscvWordProperties.
+Import TracePredicate TracePredicateNotations metric_SPI lightbulb_spec.
+
+Definition goodObservables iol (mc : MetricLogging.MetricLog) :=
+  exists ioh, metric_SPI.mmio_trace_abstraction_relation ioh iol /\
+                               goodHlTrace _ ioh.
+
+Definition lightbulb_spec : ProgramSpec := {|
+  datamem_start := MemoryLayout.heap_start ml;
+  datamem_pastend := MemoryLayout.heap_pastend ml;
+  ExprImpEventLoopSpec.goodObservables := goodObservables;
+  isReady t m := exists buf R,
+    (Separation.sep (Array.array Scalars.scalar8 (word.of_Z 1) (word.of_Z buffer_addr) buf) R) m /\
+    Z.of_nat (Datatypes.length buf) = 1520;
+|}.
+
+Import ToplevelLoop GoFlatToRiscv regs_initialized LowerPipeline.
+Require Import bedrock2.WordNotations. Local Open Scope word_scope.
+Import bedrock2.Map.Separation. Local Open Scope sep_scope.
+Require Import bedrock2.ReversedListNotations.
+Local Notation run_one_riscv_instr := (mcomp_sat (run1 Decode.RV32IM)).
+Local Notation RiscvMachine := MetricRiscvMachine.
+Local Notation run1 := (mcomp_sat (run1 Decode.RV32IM)).
+Implicit Types mach : RiscvMachine.
+Local Coercion word.unsigned : word.rep >-> Z.
+
+Definition initial_conditions mach :=
+  code_start ml = mach.(getPc) /\
+  [] = mach.(getLog) /\
+  mach.(getNextPc) = word.add mach.(getPc) (word.of_Z 4) /\
+  regs_initialized (getRegs mach) /\
+  (forall a : word32, code_start ml <= a < code_pastend ml -> In a (getXAddrs mach)) /\
+  valid_machine mach /\
+  (imem (code_start ml) (code_pastend ml) lightbulb_insns ⋆
+   mem_available (heap_start ml) (heap_pastend ml) ⋆
+   mem_available (stack_start ml) (stack_pastend ml)) (getMem mach).
+
+Lemma initial_conditions_sufficient mach :
+  initial_conditions mach ->
+  CompilerInvariant.initial_conditions compile_ext_call ml lightbulb_spec mach.
+Proof.
+  intros (? & ? & ? & ? & ? & ? & ?).
+  econstructor.
+  eexists lightbulb_insns.
+  eexists lightbulb_finfo.
+  eexists lightbulb_stack_size.
+  rewrite lightbulb_compiler_result_ok; ssplit; trivial using compiler_emitted_valid_instructions; try congruence.
+  2,3:vm_compute; inversion 1.
+  1: econstructor (* ProgramSatisfiesSpec *).
+  1: vm_compute; reflexivity.
+  1: instantiate (1:=snd init).
+  3: instantiate (1:=snd loop).
+  1,3: exact eq_refl.
+  1,2: cbv [hl_inv init loop]; cbn [fst snd]; intros; eapply MetricWeakestPreconditionProperties.sound_cmd.
+  all : repeat MetricProgramLogic.straightline.
+
+  (*
+MetricWeakestPrecondition.cmd (map.of_list funcs)
+  (snd init) [] m0 map.empty mc0
+  (fun (t : trace) (m : SortedListWord.map word32 Init.Byte.byte)
+     (_ : SortedListString.map word32) (mc : MetricLogging.MetricLog) =>
+   isReady lightbulb_spec t m /\ goodObservables lightbulb_spec t mc)
+
+========================= (2 / 2)
+
+MetricWeakestPrecondition.cmd (map.of_list funcs)
+  (snd loop) t m l mc
+  (fun (t0 : trace) (m0 : SortedListWord.map word32 Init.Byte.byte)
+     (_ : SortedListString.map word32) (mc0 : MetricLogging.MetricLog) =>
+   isReady lightbulb_spec t0 m0 /\
+   goodObservables lightbulb_spec t0 (eventLoopJumpMetrics mc0))
+   *)
+Admitted.
+
+Import OmniSmallstepCombinators.
+
+Theorem lightbulb_correct : forall mach : MetricRiscvMachine, initial_conditions mach ->
+  always run1 (eventually run1 (fun mach' => goodObservables mach'.(getLog) (MetricsToRiscv.raiseMetrics mach'.(getMetrics)))) mach.
+Proof.
+  intros ? H%initial_conditions_sufficient; revert H.
+  unshelve rapply @always_eventually_observables; trivial using ml_ok, @Naive.word32_ok.
+  { eapply (naive_word_riscv_ok 5%nat). }
+  { eapply @compile_ext_call_correct; try exact _. }
+Qed.
+
+Print Assumptions lightbulb_correct.
